x86/AsmInject.v
@@ -1,0 +1,235 @@
+(* ******************* *)
+(* Author: Yuting Wang *)
+(* Date:   May 28, 2020 *)
+(* ******************* *)
+
+(** * Properties about Injections at the Asm Level *)
+
+Require Import Coqlib Errors.
+Require Import Integers Floats AST Linking.
+Require Import Values Memory Events Globalenvs Smallstep.
+Require Import Op Locations Mach Conventions Asm AsmFacts.
+Require Import LocalLib.
+Import ListNotations.
+
+Open Scope Z_scope.
+
+(** ** Definition of injection between register sets *)
+Definition regset_inject (j:meminj) (rs rs' : regset) : Prop :=
+  forall r, Val.inject j (rs r) (rs' r).
+
+
+Lemma Pregmap_gsspec_alt : forall (A : Type) (i j : Pregmap.elt) (x : A) (m : Pregmap.t A),
+    (m # j <- x) i  = (if Pregmap.elt_eq i j then x else m i).
+Proof.
+  intros. apply Pregmap.gsspec.
+Qed.
+
+
+Lemma regset_inject_incr : forall j j' rs rs',
+    regset_inject j rs rs' ->
+    inject_incr j j' ->
+    regset_inject j' rs rs'.
+Proof.
+  unfold inject_incr, regset_inject. intros.
+  specialize (H r).
+  destruct (rs r); inversion H; subst; auto.
+  eapply Val.inject_ptr. apply H0. eauto. auto.
+Qed.
+
+Lemma undef_regs_pres_inject : forall j rs rs' regs,
+  regset_inject j rs rs' ->
+  regset_inject j (Asm.undef_regs regs rs) (Asm.undef_regs regs rs').
+Proof.
+  unfold regset_inject. intros. apply val_inject_undef_regs.
+  auto.
+Qed.    
+
+Lemma regset_inject_expand : forall j rs1 rs2 v1 v2 r,
+  regset_inject j rs1 rs2 ->
+  Val.inject j v1 v2 ->
+  regset_inject j (rs1 # r <- v1) (rs2 # r <- v2).
+Proof.
+  intros. unfold regset_inject. intros.
+  repeat rewrite Pregmap_gsspec_alt. 
+  destruct (Pregmap.elt_eq r0 r); auto.
+Qed.
+
+Lemma regset_inject_expand_vundef_left : forall j rs1 rs2 r,
+  regset_inject j rs1 rs2 ->
+  regset_inject j (rs1 # r <- Vundef) rs2.
+Proof.
+  intros. unfold regset_inject. intros.
+  rewrite Pregmap_gsspec_alt. destruct (Pregmap.elt_eq r0 r); auto.
+Qed.
+
+Lemma set_res_pres_inject : forall res j rs1 rs2,
+    regset_inject j rs1 rs2 ->
+    forall vres1 vres2,
+    Val.inject j vres1 vres2 ->
+    regset_inject j (set_res res vres1 rs1) (set_res res vres2 rs2).
+Proof.
+  induction res; auto; simpl; unfold regset_inject; intros.
+  - rewrite Pregmap_gsspec_alt. destruct (Pregmap.elt_eq r x); subst.
+    + rewrite Pregmap.gss. auto.
+    + rewrite Pregmap.gso; auto.
+  - exploit (Val.hiword_inject j vres1 vres2); eauto. intros. 
+    exploit (Val.loword_inject j vres1 vres2); eauto. intros.
+    apply IHres2; auto.
+Qed.
+
+
+Lemma nextinstr_pres_inject : forall j rs1 rs2 sz,
+    regset_inject j rs1 rs2 ->
+    regset_inject j (nextinstr rs1 sz) (nextinstr rs2 sz).
+Proof.
+  unfold nextinstr. intros. apply regset_inject_expand; auto.
+  apply Val.offset_ptr_inject. auto.
+Qed.  
+
+Lemma nextinstr_nf_pres_inject : forall j rs1 rs2 sz,
+    regset_inject j rs1 rs2 ->
+    regset_inject j (nextinstr_nf rs1 sz) (nextinstr_nf rs2 sz).
+Proof.
+  intros. apply nextinstr_pres_inject.
+  apply undef_regs_pres_inject. auto.
+Qed. 
+
+
+Lemma set_pair_pres_inject : forall j rs1 rs2 v1 v2 loc,
+    regset_inject j rs1 rs2 ->
+    Val.inject j v1 v2 ->
+    regset_inject j (set_pair loc v1 rs1) (set_pair loc v2 rs2).
+Proof.
+  intros. unfold set_pair, Asm.set_pair. destruct loc; simpl.
+  - apply regset_inject_expand; auto.
+  - apply regset_inject_expand; auto.
+    apply regset_inject_expand; auto.
+    apply Val.hiword_inject; auto.
+    apply Val.loword_inject; auto.
+Qed.
+
+Ltac solve_val_inject :=
+  match goal with
+  (* | [ H : Val.inject _ (Vint _) (Vlong _) |- _] => inversion H *)
+  (* | [ H : Val.inject _ (Vint _) (Vfloat _) |- _] => inversion H *)
+  (* | [ H : Val.inject _ (Vint _) (Vsingle _) |- _] => inversion H *)
+  (* | [ H : Val.inject _ (Vint _) (Vptr _ _) |- _] => inversion H *)
+  (* | [ H : Val.inject _ (Vptr _ _) (Vlong _) |- _] => inversion H *)
+  (* | [ H : Val.inject _ (Vptr _ _) (Vfloat _) |- _] => inversion H *)
+  (* | [ H : Val.inject _ (Vptr _ _) (Vsingle _) |- _] => inversion H *)
+  | [ H : Val.inject _ (Vfloat _) Vundef |- _] => inversion H
+  | [ H : Val.inject _ (Vfloat _) (Vint _) |- _] => inversion H
+  | [ H : Val.inject _ (Vfloat _) (Vlong _) |- _] => inversion H
+  | [ H : Val.inject _ (Vfloat _) (Vsingle _) |- _] => inversion H
+  | [ H : Val.inject _ (Vfloat _) (Vptr _ _) |- _] => inversion H
+  | [ H : Val.inject _ (Vfloat _) (Vfloat _) |- _] => inv H; solve_val_inject
+  | [ H : Val.inject _ (Vsingle _) Vundef |- _] => inversion H
+  | [ H : Val.inject _ (Vsingle _) (Vint _) |- _] => inversion H
+  | [ H : Val.inject _ (Vsingle _) (Vlong _) |- _] => inversion H
+  | [ H : Val.inject _ (Vsingle _) (Vsingle _) |- _] => inv H; solve_val_inject
+  | [ H : Val.inject _ (Vsingle _) (Vptr _ _) |- _] => inversion H
+  | [ H : Val.inject _ (Vsingle _) (Vfloat _) |- _] => inversion H
+  | [ |- Val.inject _ (Val.of_bool ?v) (Val.of_bool ?v) ] => apply Val.vofbool_inject
+  | [ |- Val.inject _ Vundef _ ] => auto
+  end.
+
+Ltac solve_regset_inject :=
+  match goal with
+  | [ H: regset_inject ?j ?rs1 ?rs2 |- regset_inject ?j (Asm.undef_regs ?uregs ?rs1) (Asm.undef_regs ?uregs ?rs2)] =>
+    apply undef_regs_pres_inject; auto
+  | [ |- regset_inject _ (Asm.undef_regs _ _) _ ] =>
+    unfold Asm.undef_regs; solve_regset_inject
+  | [ |- regset_inject _ _ (Asm.undef_regs _ _) ] =>
+    unfold Asm.undef_regs; simpl; solve_regset_inject
+  | [ |- regset_inject _ (?rs1 # ?r <- ?v1) (?rs2 # ?r <- ?v2) ] =>
+    apply regset_inject_expand; [solve_regset_inject | solve_val_inject]
+  | [ H: regset_inject ?j ?rs1 ?rs2 |- regset_inject ?j ?rs1 ?rs2 ] =>
+    auto
+  end.
+
+Lemma compare_floats_inject: forall j v1 v2 v1' v2' rs rs',
+    Val.inject j v1 v1' -> Val.inject j v2 v2' ->
+    regset_inject j rs rs' -> 
+    regset_inject j (compare_floats v1 v2 rs) (compare_floats v1' v2' rs').
+Proof.
+  intros. unfold compare_floats, Asm.compare_floats.
+  destruct v1, v2, v1', v2'; try solve_regset_inject. 
+Qed.
+
+Lemma compare_floats32_inject: forall j v1 v2 v1' v2' rs rs',
+    Val.inject j v1 v1' -> Val.inject j v2 v2' ->
+    regset_inject j rs rs' -> 
+    regset_inject j (compare_floats32 v1 v2 rs) (compare_floats32 v1' v2' rs').
+Proof.
+  intros. unfold compare_floats32, Asm.compare_floats32.
+  destruct v1, v2, v1', v2'; try solve_regset_inject. 
+Qed.
+
+Ltac solve_opt_lessdef := 
+  match goal with
+  | [ |- Val.opt_lessdef (match ?rs1 ?r with
+                     | _ => _
+                     end) _ ] =>
+    let EQ := fresh "EQ" in (destruct (rs1 r) eqn:EQ; solve_opt_lessdef)
+  | [ |- Val.opt_lessdef None _ ] => constructor
+  | [ |- Val.opt_lessdef (Some _) (match ?rs2 ?r with
+                              | _ => _
+                              end) ] =>
+    let EQ := fresh "EQ" in (destruct (rs2 r) eqn:EQ; solve_opt_lessdef)
+  | [ H1: regset_inject _ ?rs1 ?rs2, H2: ?rs1 ?r = _, H3: ?rs2 ?r = _ |- _ ] =>
+    generalize (H1 r); rewrite H2, H3; clear H2 H3; inversion 1; subst; solve_opt_lessdef
+  | [ |- Val.opt_lessdef (Some ?v) (Some ?v) ] => constructor
+  end.
+
+Lemma eval_testcond_inject: forall j c rs1 rs2,
+    regset_inject j rs1 rs2 ->
+    Val.opt_lessdef (Asm.eval_testcond c rs1) (Asm.eval_testcond c rs2).
+Proof.
+  intros. destruct c; simpl; try solve_opt_lessdef.
+Qed.
+
+
+Section WITHMEMORYMODEL.
+  
+Context `{memory_model: Mem.MemoryModel }.
+Existing Instance inject_perm_all.
+
+
+Lemma compare_ints_inject: forall j v1 v2 v1' v2' rs rs' m m',
+    Val.inject j v1 v1' -> Val.inject j v2 v2' ->
+    Mem.inject j (def_frame_inj m) m m' ->
+    regset_inject j rs rs' -> 
+    regset_inject j (compare_ints v1 v2 rs m) (compare_ints v1' v2' rs' m').
+Proof.
+  intros. unfold compare_ints, Asm.compare_ints.
+  repeat apply regset_inject_expand; auto.
+  - apply cmpu_inject; auto.
+  - apply cmpu_inject; auto.
+  - apply val_negative_inject. apply Val.sub_inject; auto.
+  - apply sub_overflow_inject; auto.
+Qed.
+
+Lemma compare_longs_inject: forall j v1 v2 v1' v2' rs rs' m m',
+    Val.inject j v1 v1' -> Val.inject j v2 v2' ->
+    Mem.inject j (def_frame_inj m) m m' ->
+    regset_inject j rs rs' -> 
+    regset_inject j (compare_longs v1 v2 rs m) (compare_longs v1' v2' rs' m').
+Proof.
+  intros. unfold compare_longs, Asm.compare_longs.
+  repeat apply regset_inject_expand; auto.
+  - unfold Val.cmplu.
+    exploit (cmplu_bool_lessdef j v1 v2 v1' v2' m m' Ceq); eauto. intros.
+    inversion H3; subst.
+    + simpl. auto. 
+    + simpl. apply Val.vofbool_inject.
+  - unfold Val.cmplu.
+    exploit (cmplu_bool_lessdef j v1 v2 v1' v2' m m' Clt); eauto. intros.
+    inversion H3; subst.
+    + simpl. auto. 
+    + simpl. apply Val.vofbool_inject.
+  - apply val_negativel_inject. apply Val.subl_inject; auto.
+  - apply subl_overflow_inject; auto.
+Qed.
+
+End WITHMEMORYMODEL.
