Makefile
@@ -126,7 +126,7 @@ BACKEND=\
   RelocProgSemantics.v RelocProgSemantics1.v RelocProgSemantics2.v RelocProgSemantics3.v \
   TablesEncodeproof.v \
   RelocBinDecode.v \
-  LocalLib.v
+  LocalLib.v AsmInject.v
 
 
 
